# Hoare Logic
- {p} S {q}
	- precondition, program segment, postcondition
	- e.g. $\{x+1\leq2022\}{x{\leftarrow}x+1}\{x\leq2022\}$ 
# Induction
- EWWWWWWWWWWW
- General Form
	- ![[Pasted image 20221103140626.png|500]]
		- $P(n)$ is a predicate (true/false statement)
		- Prove $P(n_0)$, then prove that with $P(n)$, $P(n+1)$ is true. That proves from $n_0$ to all that follows.
		- If you didn't use 
## Ex
- ![[Pasted image 20221103141132.png|450]]
## Ex (Classic 321 $i^2$ summation prove)
- ![[Pasted image 20221103143657.png|400]]
- This concludes the proof by induction $\square$ wow
## Ex (correctness)
	1 p <-- 1
	2 for i <-- 1 to k
	3 	p <-- p * x
	4 return p
- Claim: After the $i$th iteration, $p=x^i$ for $i\geq1$ 
	- Underline is called Loop Invariant
- Proof: By induction on $i$
	- $P(i)=x^i$
	- $P(1)=x^1=x$
	- $P(i+1)=x^{i+1}$
- Base Case: $P(i+1)=x^{i+1}$, this is true because line 1: p <-- 1.
- Ind Hypothesis: Assume that $P(i)=x^i$ for some $i\geq1$
- Ind Step: We need to show $P(i+1)=x^{i+1}$
	- This holds because after the ith iteration, $p=x^i$ (Ind Hypo).
	- Then in the $(i+1)$th iteration, on line 3, $p$ becomes $p*x$, which is $x^1*x$ which is $x^{i+1}$
## Ex (correctness HW4)
<u>Claim</u>: After the $j^\text{th}$ iteration, $d = a^{j} \bmod m$ for $j \geq 1$
<u>Proof</u>: By induction on $j$.
- After the $j^\text{th}$ iteration, $d = a^{j} \bmod m$
- After the 1st iteration, $d = a^{1}\bmod m = a \bmod m$
- After the $(j+1)^\text{th}$ iteration, $d = a^{j+1} \bmod m$
<u>Base Case</u>: After the 1st iteration, $d = a^{1} \bmod m = a\bmod m$.
- This is true because:
	- On line 1, $d$ is set to 1.
	- Then we go it goes into the loop for the 1st time on line 6.
		- Line 6 modifies $d$ to $(d*a) \bmod m = (1*a) \bmod m = a \bmod m$
<u>IH</u>: Assume that after the $j^\text{th}$ iteration, $d = a^{j} \bmod m$ for some $j\geq1$
<u>IS</u>: We need to show that After the $(j+1)^\text{th}$, $d = a^{j+1} \bmod m$
- We know that after the $j^\text{th}$ iteration, $d = a^{j} \bmod m$ \[IH]
- So when it enters the loop again:
	- Line 6 modifies $d$ to 
		$\begin{align} (d*a) \bmod m &= ((a^{j} \bmod m) * a) \bmod m \text{ [Lemma 1]} \\ &= a^{j} a \bmod m \\ &= a^{j+1} \bmod m \end{align}$
	- proving the claim true by induction.
- Lemma 1: (from Binary Exponentiation)
	 $\begin{align} ((a \bmod m)b) \bmod m &= (((a \bmod m) \bmod m) (b \bmod m)) \bmod m \\ &= ((a \bmod m) (b \bmod m)) \bmod m \\ &= (ab) \bmod m\end{align}$
## Ex (Ian ez)
	1 S <- 0
	2 for i <- 1 to n do
	3 	S <- S + i * i
	4 return S
<u>Claim</u>: After the $j^\text{th}$ iteration, $S=\sum_{i=1}^{n}i^{2}$, $n \geq 1$.
<u>Base Case</u>: After the 1st iteration, $S=\sum_{i=1}^{n}1^{2}=1$,
- This is true because:
	- Line 1 sets $S=0$
	- We 1st enter the loop on line 2 with $i=1$
		- Line 3 modifies $S$ into $S+i^2=0+1^2=1$
<u>IH</u>: Assume that after $j^\text{th}$ iterations, $S=\sum_{i=1}^{n}i^{2} = \frac{n\left(n+1\right)\left(2n+1\right)}{6}$, for some $n \geq 1$.
<u>IS</u>: We need to show that after the $(j+1)^\text{th}$ iteration, $S=\sum_{i=1}^{n+1}i^{2} = \sum_{i=1}^{n}i^{2}+\sum_{i=n+1}^{n+1}i^{2} = \frac{\left(n+1\right)\left(n+2\right)\left(2n+3\right)}{6}$
- We know that after the $j^\text{th}$ iteration, $S=\sum_{i=1}^{n}i^{2}$ \[IH]
- So when we enter the loop again: 
	- Line 3 modifies S into
		$\begin{align} S+i^{2} &= \left(\sum_{i=1}^{n}i^{2}\right)+i^{2} \\ &= \frac{n\left(n+1\right)\left(2n+1\right)}{6} +i^2 \end{align}$
## Ex
- Proof: $2n+3\leq2^n$ for all $n>3$
- Claim: $2n+3\leq2^n$ for all $n>3$
- Proof: by induction on n
	- $P(n)=2n+3\leq2^n$
	- $P(4) = 2(4)+3\leq2^{4} \iff 11\leq16$
	- $P(n+1) = 2(n+1)+3 \leq 2^{n+1}$
- Base Case: $P(4) = 2(4)+3\leq2^{4} \iff 11\leq16$
- IH:  $P(n)=2n+3\leq2^n$ for some $n>3$
- IS: We need to show $P(n+1) = 2(n+1)+3 \leq 2^{n+1}$
	- $2(n+1)+3 \leq 2^{n+1}$
	- $2n+2+3 \leq 2^n*2^1$
	- $2n+5 \leq 2^n*2^1$
	- $2n+{5/2} \leq 2^n$
	- Bruh, find the order and use IH
# Psuedopolymonial
- When the algorithm is linear in the 